Kura/Graph/Subgraph.lean
@@ -6,291 +6,40 @@ open edge
 variable {V W E F : Type*} [LinearOrder V] [LinearOrder W]
 
 
-/--
-If removeV v = true, v is removed when InducedSubgraph is evaluated-/
-structure InducedSubgraph (G : Graph V E) where
-  Vset : Set V
-  DecVMem : DecidablePred (· ∈ Vset)
+-- one op?
+def Vs (G : Graph V E) (S : Set V) [DecidablePred (· ∈ S)] : Graph S {e // G.all e (· ∈ S) } where
+  inc e :=
+    let ⟨e, he⟩ := e
+    edge.pmap Subtype.mk (G.inc e) (by
+    intro v hv
+    simp only [all, all_iff, decide_eq_true_eq] at he
+    exact he v hv)
 
-structure Subgraph (G : Graph V E) extends InducedSubgraph G where
-  Eset : Set E
-  DecEMem : DecidablePred (· ∈ Eset)
-  Eset_spec : ∀ e ∈ Eset, ∀ v ∈ G.inc e, v ∈ Vset
+macro G:term "[" S:term "]ᴳ" : term => `(Graph.Vs $G $S)
 
-structure QuotientGraph (G : Graph V E) where
-  vmap : V → V
-  vmap_idem : ∀ v, vmap (vmap v) = vmap v
+def Es (G : Graph V E) (S : Set E) [DecidablePred (· ∈ S)] : Graph V S where
+  inc := (G.inc ·.val)
 
-/-- If v is mapped to ⊥ = none, remove it -/
-structure QuotientSubgraph (G : Graph V E) where
-  vmap' : V → WithBot V
-  vmap'_idem : ∀ v, Option.bind (vmap' v) vmap' = vmap' v
-  Eset : Set E
-  DecEMem : DecidablePred (· ∈ Eset)
-  Eset_spec : ∀ e ∈ Eset, ∀ v ∈ G.inc e, (vmap' v).isSome
-
-----------------------------------------------------------------------
--- useful lemma
-
-variable {G : Graph V E}
-
-lemma Subgraph.not_mem_Eset  (S : Subgraph G) (he : ∃ v ∈ G.inc e, v ∉ S.Vset) :
-    e ∉ S.Eset := by
-  intro h
-  absurd S.Eset_spec e h
-  push_neg
-  exact he
-
-lemma QuotientSubgraph.not_mem_Eset (S : QuotientSubgraph G) (he : ∃ v ∈ G.inc e, (S.vmap' v).isNone) :
-    e ∉ S.Eset := by
-  intro h
-  absurd S.Eset_spec e h
-  push_neg
-  simpa only [ne_eq, Bool.not_eq_true, Option.not_isSome, Option.isNone_iff_eq_none] using he
-
-/-- Expose the decidability of (· ∈ Vset) -/
-instance InducedSubgraphDecVMem {G : Graph V E} (S : InducedSubgraph G) :
-    DecidablePred (· ∈ S.Vset) := S.DecVMem
-
-/-- Expose the decidability of (· ∈ Eset)-/
-instance SubgraphDecEMem (S : Subgraph G) : DecidablePred (· ∈ S.Eset) := S.DecEMem
-
-/-- Make vmap_idem simp-avaliable-/
-@[simp]
-lemma QuotientGraph.vmap_idem_for_simp  (S : QuotientGraph G) (v : V) :
-    S.vmap (S.vmap v) = S.vmap v := S.vmap_idem v
-
-/-- Expose the decidability of (· ∈ Eset)-/
-instance QuotientSubgraphDecEMem (S : QuotientSubgraph G) : DecidablePred (· ∈ S.Eset) := S.DecEMem
-
--------------------------------------------------
--- Evaluations
-
-def InducedSubgraph.eval (S : InducedSubgraph G) :
-  Graph S.Vset {e // (G.inc e).all (· ∈ S.Vset) } where
-  inc e := edge.pmap Subtype.mk (G.inc e.1) (by
-    simpa only [all_iff, decide_eq_true_eq] using e.prop)
-
-def Subgraph.eval (S : Subgraph G) :
-  Graph S.Vset S.Eset where
-  inc e := edge.pmap Subtype.mk (G.inc e.1) (S.Eset_spec e.val e.prop)
-
--- some setup is needed to make this work for QuotientGraph
-def QuotientGraph.ran (S : QuotientGraph G) : Set V :=
-  {v | ∃ u, S.vmap u = v}
-
-lemma QuotientGraph.mem_ran_iff (S : QuotientGraph G) (v : V) :
-    v ∈ S.ran ↔ ∃ u, S.vmap u = v := Iff.rfl
-
-@[simp]
-lemma QuotientGraph.mem_ran_iff_vmap_self (S : QuotientGraph G) (v : V) :
-    v ∈ S.ran ↔ S.vmap v = v := by
-  rw [QuotientGraph.mem_ran_iff]
-  constructor
-  · rintro ⟨ u, hu ⟩
-    rw [← hu]
-    exact S.vmap_idem u
-  · rintro h
-    exact ⟨ v, h ⟩
-
-def QuotientGraph.vmapRan (S : QuotientGraph G) (v : V) : S.ran :=
-  ⟨ S.vmap v, by rw [mem_ran_iff_vmap_self, vmap_idem_for_simp]⟩
-
-def QuotientGraph.eval (S : QuotientGraph G) : Graph (S.ran) E where
-  inc e := (G.inc e).map S.vmapRan
-
--- Even more setup is needed to make this work for QuotientSubgraph
-def QuotientSubgraph.ran (S : QuotientSubgraph G) : Set V :=
-  {v | ∃ u, S.vmap' u = some v}
-
-def QuotientSubgraph.Vset (S : QuotientSubgraph G) : Set V :=
-  {v | (S.vmap' v).isSome }
-
-@[simp]
-lemma QuotientSubgraph.mem_Vset_iff (S : QuotientSubgraph G) (v : V) :
-    v ∈ S.Vset ↔ (S.vmap' v).isSome := Iff.rfl
-
-/-- if e is in Eset, all vertices incident to e is not removed.
-  Embed this fact to the type of each v. -/
-def QuotientSubgraph.domSubtype (S : QuotientSubgraph G) (e : S.Eset) : edge S.Vset :=
-  (G.inc e).pmap Subtype.mk (fun v hv => S.Eset_spec e.val e.prop v hv)
-
-def QuotientSubgraph.vmap'Ran (S : QuotientSubgraph G) (v : S.Vset) : S.ran :=
-  ⟨ (S.vmap' v.val).get v.prop, by simp only [ran, Set.mem_setOf_eq, Option.some_get,
-    exists_apply_eq_apply]⟩
-
-def QuotientSubgraph.eval (S : QuotientSubgraph G) : Graph S.ran S.Eset where
-  inc e := S.domSubtype e |>.map S.vmap'Ran
-
-------------------------------------------------------------------------
--- Carrying over the instances
-
-instance InducedSubgraphFullgraph [fullGraph G] (S : InducedSubgraph G) :
-  fullGraph (V := S.Vset) S.eval where
-  all_full := sorry
-
-instance SubgraphFullgraph [fullGraph G] (S : Subgraph G) :
-  fullGraph (V := S.Vset) S.eval where
-  all_full := sorry
-
-instance QuotientGraphFullgraph [fullGraph G] (S : QuotientGraph G) :
-  fullGraph (V := S.ran) S.eval where
-  all_full := sorry
-
-instance QuotientSubgraphFullgraph [fullGraph G] (S : QuotientSubgraph G) :
-  fullGraph (V := S.ran) S.eval where
-  all_full := sorry
-
-instance InducedSubgraphUndirected [Undirected G] (S : InducedSubgraph G) :
-  Undirected (V := S.Vset) S.eval where
-  edge_symm := sorry
-
-instance SubgraphUndirected [Undirected G] (S : Subgraph G) :
-  Undirected (V := S.Vset) S.eval where
-  edge_symm := sorry
-
-instance QuotientGraphUndirected [Undirected G] (S : QuotientGraph G) :
-  Undirected (V := S.ran) S.eval where
-  edge_symm := sorry
-
-instance QuotientSubgraphUndirected [Undirected G] (S : QuotientSubgraph G) :
-  Undirected (V := S.ran) S.eval where
-  edge_symm := sorry
-
------------------------------------------------------------------------------
--- Initializations
-
-variable (G : Graph V E)
-
-def InducedSubgraph.init : InducedSubgraph G where
-  Vset := Set.univ
-  DecVMem := by infer_instance
-
-def Subgraph.init : Subgraph G where
-  Vset := Set.univ
-  DecVMem := by infer_instance
-  Eset := Set.univ
-  DecEMem := by infer_instance
-  Eset_spec := by simp only [Set.mem_univ, implies_true, imp_self]
-
-def QuotientGraph.init : QuotientGraph G where
-  vmap := id
-  vmap_idem := fun _ => rfl
-
-def QuotientSubgraph.init : QuotientSubgraph G where
-  vmap' := some
-  vmap'_idem := by simp only [Option.bind_some, implies_true]
-  Eset := Set.univ
-  DecEMem := by infer_instance
-  Eset_spec := by simp only [Set.mem_univ, Option.isSome_some, implies_true, imp_self]
-
------------------------------------------------------------------------------
--- Elementary operations
-
-variable {G : Graph V E}
-
-def InducedSubgraph.vrm (G' : InducedSubgraph G) (v : V) : InducedSubgraph G where
-  Vset := G'.Vset \ {v}
-  DecVMem := by infer_instance
-
-def InducedSubgraph.OnSet (G' : InducedSubgraph G) (S : Set V) [DecidablePred (· ∈ S)] :
-    InducedSubgraph G where
-  Vset := G'.Vset ∩ S
-  DecVMem := by infer_instance
-
-macro G:term "[" S:term "]ᴳ" : term =>
-  `(InducedSubgraph.eval (InducedSubgraph.OnSet (InducedSubgraph.init $G) $S))
+macro G:term "{" S:term "}ᴳ" : term => `(Graph.Es $G $S)
 
 
-def Subgraph.vrm (G' : Subgraph G) (v : V) : Subgraph G where
-  Vset := G'.Vset \ {v}
-  DecVMem := by infer_instance
-  Eset := {e ∈ G'.Eset | G.all e (· ≠ v)}
-  DecEMem := by infer_instance
-  Eset_spec e he u hu := by
-    simp only [all, ne_eq, decide_not, all_iff, Bool.not_eq_true', decide_eq_false_iff_not,
-      Set.mem_setOf_eq, Set.mem_diff, Set.mem_singleton_iff] at he ⊢
-    constructor
-    · exact G'.Eset_spec e he.1 u hu
-    · exact he.2 u hu
+def Qs (G : Graph V E) (S : Set V) [DecidablePred (· ∈ S)] (v : V) (hv : v ∉ S) :
+  Graph (Sᶜ:Set _) E where
+  inc e := G.inc e
+    |>.map (fun u => if u ∈ S then v else u)
+    |>.pmap Subtype.mk (fun w hw => by
+      simp only [mem_map_iff] at hw
+      obtain ⟨u, _hu, rfl⟩ := hw
+      split
+      · exact hv
+      · assumption)
 
-def Subgraph.OnSetV (G' : Subgraph G) (S : Set V) [DecidablePred (· ∈ S)] : Subgraph G where
-  Vset := G'.Vset ∩ S
-  DecVMem := by infer_instance
-  Eset := {e ∈ G'.Eset | G.all e (· ∈ S)}
-  DecEMem := by infer_instance
-  Eset_spec e he u hu := by
-    simp only [all, all_iff, decide_eq_true_eq, Set.mem_setOf_eq, Set.mem_inter_iff] at he ⊢
-    constructor
-    · exact G'.Eset_spec e he.1 u hu
-    · exact he.2 u hu
+-- Merges to the start of the path
+def Ms (G : Graph V E) [DecidableEq E] (P : G.Path) :
+    Graph {v : V // v ∉ P.vertices.tail} {e : E // e ∉ P.edges} where
+  inc e := G
+    |>.Qs {v : V | v ∈ P.vertices.tail} P.start P.start_not_mem_vertices_tail
+    |>.Es {e : E | e ∉ P.edges}
+    |>.inc e
 
-def Subgraph.erm [DecidableEq E] (G' : Subgraph G) (e : E) : Subgraph G where
-  Vset := G'.Vset
-  DecVMem := by infer_instance
-  Eset := G'.Eset \ {e}
-  DecEMem := by infer_instance
-  Eset_spec e' he' u hu := by
-    simp only [Set.mem_diff, Set.mem_singleton_iff] at he'
-    exact G'.Eset_spec e' he'.1 u hu
-
-def Subgraph.OnSetE (G' : Subgraph G) (S : Set E) [DecidablePred (· ∈ S)] : Subgraph G where
-  Vset := G'.Vset
-  DecVMem := by infer_instance
-  Eset := G'.Eset ∩ S
-  DecEMem := by infer_instance
-  Eset_spec e he u hu := by
-    simp only [Set.mem_inter_iff] at he
-    exact G'.Eset_spec e he.1 u hu
-
-macro G:term "{" S:term "}ᴳ" : term => `(Subgraph.eval (Subgraph.OnSetE (Subgraph.init $G) $S))
-
-/-- The second vertex is being merged into the first vertex-/
-def QuotientGraph.merge (G' : QuotientGraph G) (v w : V) :
-    QuotientGraph G where
-  vmap u := if G'.vmap u = w then G'.vmap v else G'.vmap u
-  vmap_idem u := by
-    by_cases hu : G'.vmap u = w <;> simp only [hu, ↓reduceIte, vmap_idem_for_simp, ite_self]
-
-def QuotientGraph.mergeOnSet (G' : QuotientGraph G) (S : Set V) [DecidablePred (· ∈ S)] (x : V) :
-    QuotientGraph G where
-  vmap u := if G'.vmap u ∈ S then G'.vmap x else G'.vmap u
-  vmap_idem u := by
-    by_cases hu : G'.vmap u ∈ S <;> simp only [hu, ↓reduceIte, vmap_idem_for_simp, ite_self]
-
-
-def QuotientSubgraph.vrm [DecidableEq E] (G' : QuotientSubgraph G) (v : V) :
-    QuotientSubgraph G where
-  vmap' u := if G'.vmap' u = v then ⊥ else G'.vmap' u
-  vmap'_idem u := by
-    by_cases hu : G'.vmap' u = v <;> simp [hu, ↓reduceIte]
-    · rfl
-    · by_cases hvu : (G'.vmap' u) = none
-      · simp only [hvu, Option.none_bind]
-      · obtain ⟨w, hw⟩ := Option.ne_none_iff_exists.mp hvu
-        simp only [← hw, Option.some_bind]
-        sorry
-  Eset := {e ∈ G'.Eset | G.all e (G'.vmap' · ≠ v)}
-  DecEMem := by infer_instance
-  Eset_spec e he u hu := by
-    simp only [ne_eq, decide_not, all_iff, Bool.not_eq_true', decide_eq_false_iff_not,
-      Set.mem_setOf_eq] at he
-    simp only [he.2 u hu, ↓reduceIte]
-    exact G'.Eset_spec e he.1 u hu
-
-------------------------------------------------------------------------
--- Lemmas about the elementary operations
-
-lemma Subgraph.not_mem_erm [DecidableEq E] [fullGraph G] (G' : Subgraph G) (e : E) :
-    let G'' := G'.erm e
-    ¬ (e ∈ G''.Eset ∧ (G.inc e).all (· ∈ G''.Vset)) := by
-  simp only [all_iff, decide_eq_true_eq, not_and, not_forall, Classical.not_imp]
-  rintro h
-
-  sorry
-
--- def deleteEdges (G: Graph V E) (S : Set E) [DecidablePred (· ∈ S)] : Subgraph G :=
---   (Subgraph.init G).OnSetE Sᶜ
-
-
-end Graph
+-- contraction by a rooted tree?
